@prefix owl: <http://www.w3.org/2002/07/owl#> .
@prefix rdfs: <http://www.w3.org/2000/01/rdf-schema#> .
@prefix dct: <http://purl.org/dc/terms/> .
@prefix dctype: <http://purl.org/dc/dcmitype/> .
@prefix ids: <https://w3id.org/idsa/core/> .
@prefix idsm: <https://w3id.org/idsa/metamodel/> .
@prefix skos: <http://www.w3.org/2004/02/skos/core#> .
@prefix xsd: <http://www.w3.org/2001/XMLSchema#> .


# Top-level content classes
# -------------------------

ids:Data
    a owl:Class;
    # ISO 19115: identifiable collection of data
    rdfs:subClassOf ids:DigitalContent, dctype:Dataset ;
    rdfs:label "Data"@en ;
    rdfs:comment "Custom or generic (semi)structured data intended for machine processing, i.e. atomic values or arrangements of data fields (optionally defined by a schema)."@en .


ids:Text a owl:Class; # .. or "Document" ?
    # language is mandatory
    rdfs:subClassOf ids:DigitalContent, dctype:Text ;
    rdfs:label "Text"@en ;
    rdfs:comment "Informative textual content intended for reading and interpretation by humans and other intelligent agents. Comprises any digital representation of text, e.g. document and image (screenshot)."@en ;
    skos:note "Text generlizes the notion of Media Type 'text' as a meaningful sequence of characters written in a set of human language(s), regardless of the formating and file type (e.g. plain, Word or PostScript)."@en ;
    rdfs:seeAlso <https://tools.ietf.org/html/rfc2046#section-4.1> .

ids:Audio a owl:Class;
    # language is optional
    rdfs:subClassOf ids:DigitalContent, dctype:Sound ;
    rdfs:label "Audio"@en ;
    rdfs:comment "Content intended for auditive perception, requires an audio output device (i.e. a loudspeaker) to present the contents.";
    rdfs:seeAlso <https://tools.ietf.org/html/rfc2046#section-4.3> .

ids:Image a owl:Class;
    rdfs:subClassOf ids:DigitalContent, dctype:StillImage ;
    rdfs:label "Image";
    rdfs:comment "Static content intended for visual perception/interpretation, requires a display device (i.e. a screen) to present the contents.";
    rdfs:seeAlso <https://tools.ietf.org/html/rfc2046#section-4.2> .

ids:Video
    # language is optional
    a owl:Class;
    rdfs:subClassOf ids:DigitalContent, dctype:MovingImage ;
    rdfs:label "Video";
    rdfs:comment "Dynamic content intended for visual and auditive perception, combines requirements of image and audio Content Types, while imposing further requirements on video decoding etc.";
    rdfs:seeAlso <https://tools.ietf.org/html/rfc2046#section-4.4> .

ids:Software # .. or "Code" ?
    a owl:Class;
    rdfs:subClassOf ids:DigitalContent, dctype:Software ;
    rdfs:label "Software"@en ;
    rdfs:comment "Executable software (binary), interpreted program code (source) or fragments thereof. Intended purpose is an optional preprocessing (i.e. compilation, installation) and subsequnt execution/invokation of the software."@en ;
    skos:note "Term 'application' was misleading, since Mime Type of same name refers to unspecified data processed by some type of application program."@en ;
    rdfs:seeAlso <https://tools.ietf.org/html/rfc2046#section-4.5> ;
    .

ids:Container a owl:Class;
   rdfs:subClassOf ids:DigitalContent, dctype:Collection ; # ISO-19115 "aggregate"; Multipart
   rdfs:label "Container";
   rdfs:comment "Container composed of multiple (individually defined) parts.";
   rdfs:seeAlso <https://tools.ietf.org/html/rfc2046#section-5.1> ;
   .

ids:OpaqueContent a owl:Class;
   rdfs:subClassOf ids:DigitalContent ;
   rdfs:label "Opaque content";
   rdfs:comment "Opaque, not further specified type of custom, binary content."@en ;  
   .

# Derived content classes
# -----------------------

# Data
# ----

ids:AtomicData
    a owl:Class;
    rdfs:subClassOf ids:Data ;
    owl:disjointWith ids:Structure ;
    rdfs:label "Atomic data"@en ;
    rdfs:comment "Terminal data nodes, i.e. an atomic, possibly typed scalars."@en .

ids:Structure
    a owl:Class;
    rdfs:subClassOf ids:Data ;
    owl:disjointWith ids:AtomicData ;
    rdfs:label "Structure"@en ;
    rdfs:comment "Custom or standardized structured data"@en ;
    rdfs:seeAlso <https://schema.org/StructuredValue> .

ids:Collection
    a owl:Class;
    rdfs:subClassOf ids:Structure ;
    rdfs:label "Collection"@en ;
    rdfs:comment "Group of elements supporting particular access operations based on the concrete subclass."@en ;
    rdfs:seeAlso <https://docs.oracle.com/javase/8/docs/technotes/guides/collections/overview.html> .

ids:Map a owl:Class;
    rdfs:subClassOf ids:Collection ;
    rdfs:label "Map"@en ;
    rdfs:comment "Collection of elements allowing for a key based access."@en ;
    rdfs:seeAlso <https://docs.oracle.com/javase/8/docs/api/java/util/Map.html> .
    # adds keyType;

ids:List a owl:Class;
    rdfs:subClassOf ids:Collection ;
    rdfs:label "List"@en ;
    rdfs:comment "Ordered collection of elements allowing for an index-based access."@en ;
    rdfs:seeAlso <https://docs.oracle.com/javase/8/docs/api/java/util/List.html> .
    # minIndex: 0 or 1 based etc.

ids:SortOrder a owl:Class;
    rdfs:label "Sort Order"@en ;
    rdfs:comment "Class of possible order methods for collections."@en.

# Renamed from orderPolicy
ids:sortOrder a owl:ObjectProperty;
    rdfs:label "sort order"@en;
    rdfs:domain ids:List;
    rdfs:range ids:SortOrder;
    rdfs:comment "Indicates the sort order of a List."@en.

# obsolate - concept reused for inline representation instance
#ids:Value a owl:Class;
#    rdfs:subClassOf ids:Data ;
#    owl:disjointWith ids:Structure ;
#    rdfs:label "Value"@en ;
#    rdfs:comment "Terminal data node, i.e. an atomic, possibly typed scalar."@en .

# common scalar types
#ids:NumericValue a owl:Class;
#    rdfs:subClassOf ids:Value ;
#    rdfs:label "Numeric value"@en ;
#    rdfs:comment "Numeric value."@en .

#ids:BooleanValue a owl:Class;
#    rdfs:subClassOf ids:Value ;
#    rdfs:label "Boolean value"@en ;
#    rdfs:comment "Boolean value."@en .

#ids:StringValue a owl:Class;
#    rdfs:subClassOf ids:Value ;
#    rdfs:label "String value"@en ;
#    rdfs:comment "String value."@en .

#ids:Record
#    a owl:Class;
#    rdfs:subClassOf ids:Structure ;
#    rdfs:label  "Record"@en ;
#    rdfs:comment "Named arrangement of fields (possibly named, ordered, strongly typed etc.)."@en .

#ids:TabularData
#    a owl:Class;
#    rdfs:subClassOf ids:Structure ;
#    rdfs:label "Table"@en ;
#    rdfs:comment "Tabular / relational data structure."@en .

#ids:DataCube
#    a owl:Class;
#    rdfs:subClassOf ids:Structure ;
#    rdfs:label "Data cube"@en;
#    rdfs:comment "n-dimensional data structure"@en .

# Software
# --------

#ids:Schema a owl:Class; -> moved to ContentType
#    rdfs:subClassOf ids:Software ;
#    rdfs:label "Schema"@en ;
#    rdfs:comment "Machine-processable instructions defining a set of conformant, valid Serializations of a Content."@en .

#ids:XMLSchema a owl:Class;
#    rdfs:subClassOf ids:Schema ;
#    rdfs:label "XML Schema (v1.1)";
#    rdfs:comment "XML Schema Definition Language, version 1.1";
#    rdfs:isDefinedBy <https://www.w3.org/TR/xmlschema11-1/> ; # Structure
#    rdfs:isDefinedBy <https://www.w3.org/TR/xmlschema11-2/> . # Datatype
#    # ids:targetMediaType idsc_media:text_xml, idsc_media:application_xml . # Applies to XML-based media types

#ids:SchematronSchema a owl:Class;
#    rdfs:subClassOf ids:Schema ;
#    rdfs:label "Schematron";
#    rdfs:comment "Schematron schema language for XML";
#    rdfs:isDefinedBy <https://www.iso.org/standard/74515.html> ; # ISO/IEC 19757-3:2016
#    rdfs:seeAlso <http://schematron.com/> .
#    # ids:targetMediaType idsc_media:text_xml, idsc_media:application_xml . # Applies to XML-based media types

#ids:RelaxNGSchema a owl:Class;
#    rdfs:subClassOf ids:Schema ;
#    rdfs:label "Relax NG";
#    rdfs:comment "Relax NG schema language for XML";
#    rdfs:isDefinedBy <https://www.iso.org/standard/52348.html> ; # ISO/IEC 19757-2:2008
#    rdfs:seeAlso <http://www.relaxng.org/> .
#    # ids:targetMediaType idsc_media:text_xml, idsc_media:application_xml . # Applies to XML-based media types

#ids:JSONSchema a owl:Class;
#    rdfs:subClassOf ids:Schema ;
#    rdfs:label "JSON Schema";
#    rdfs:comment "JSON-based schema language for describing the structure of JSON data.";
#    rdfs:isDefinedBy <https://tools.ietf.org/id/draft-handrews-json-schema> ;
#    rdfs:seeAlso <http://json-schema.org/specification> .
#    # ids:targetMediaType idsc_media:application_json . # Applies to JSON-based media types

ids:softwareInterface
    a owl:ObjectProperty;
    rdfs:label "software interface"@en;
    rdfs:domain ids:Software;
    rdfs:range ids:Interface;
    rdfs:comment "Interface exposed by the Software, e.g. for configuration, data processing etc."@en.


ids:icon a owl:DatatypeProperty;
    rdfs:domain ids:Software;
    rdfs:range xsd:string;
    rdfs:label "Software icon"@en;
    rdfs:comment "Data-URL containing the software icon data according to RFC 2397."@en;
    rdfs:seeAlso <https://tools.ietf.org/html/rfc2397> ;
    idsm:issue "Designing icons as data-URLs makes them 'self-contained', as no referential and resolvable addresses is assumed. This may result in  a considerable amount of data enclosed in meta-data annotation."@en;
    .
