@prefix owl: <http://www.w3.org/2002/07/owl#> .
@prefix rdf:   <http://www.w3.org/1999/02/22-rdf-syntax-ns#> .
@prefix rdfs: <http://www.w3.org/2000/01/rdf-schema#> .
@prefix xsd: <http://www.w3.org/2001/XMLSchema#> .
@prefix dct: <http://purl.org/dc/terms/> .
@prefix ids: <https://w3id.org/idsa/core/> .
@prefix idsm: <https://w3id.org/idsa/metamodel/> .

# Classes
# -------

# Basic Message Types
# -------------------

ids:RequestMessage a owl:Class;
    rdfs:subClassOf ids:Message ;
    idsm:abstract true;
    rdfs:label "Request Message"@en ;
    rdfs:comment "Client-generated message initiating a communication, motivated by a certain reason and with an answer expected."@en.

ids:ResponseMessage a owl:Class;
    rdfs:subClassOf ids:Message ;
    idsm:abstract true;
    rdfs:label "Response Message"@en ;
    rdfs:comment "Response messages hold information about the reaction of a recipient to a formerly sent command or event. They must be correlated to this message."@en;
    idsm:validation [
        idsm:forProperty ids:correlationMessage;
        idsm:constraint idsm:NotNull;
    ].

ids:NotificationMessage a owl:Class ;
    rdfs:subClassOf ids:Message ;
    idsm:abstract true;
    rdfs:label "Notification Message"@en ;
    rdfs:comment "Event messages are informative and no response is expected by the sender."@en.

ids:CommandMessage a owl:Class;
    rdfs:subClassOf ids:RequestMessage ;
    idsm:abstract true;
    rdfs:label "Command Message"@en ;
    rdfs:comment "Command messages are usually sent when a response is expected by the sender. Changes state on the recipient side. Therefore, commands are not 'safe' in the sense of REST."@en.

ids:QueryMessage a owl:Class ;
    rdfs:subClassOf ids:RequestMessage ;
    idsm:abstract true;
    rdfs:label "Query Command"@en ;
    rdfs:comment "Query commands are intended to annotate query strings in a specified query language or address a specific resource."@en.

ids:ResultMessage a owl:Class;
    rdfs:subClassOf ids:ResponseMessage ;
    rdfs:label "Result Message"@en ;
    rdfs:comment "Result messages are intended to annotate the results of a query command. "@en.

ids:RejectionMessage a owl:Class;
    rdfs:subClassOf ids:ResponseMessage ;
    rdfs:label "Rejection Message"@en ;
    rdfs:comment "Rejection messages are specialized response messages that notify the sender of a message that processing of this message has failed."@en.

ids:RejectionReason a owl:Class;
    rdfs:label "RejectionReason"@en ;
    rdfs:comment "Class of reasons that might lead to issuing a Rejection message."@en.

ids:rejectionReason a owl:ObjectProperty;
    rdfs:domain ids:RejectionMessage;
    rdfs:range ids:RejectionReason;
    rdfs:label "rejectionReason"@en;
    rdfs:comment "Specifies the reason of the rejection."@en.

# Self-description Access
# -----------------------

ids:SelfDescriptionRequest a owl:Class;
    rdfs:subClassOf ids:RequestMessage ;
    rdfs:label "Self Description Request"@en ;
    rdfs:comment "Message requesting the self-description of an Infrastructure Component."@en.

ids:SelfDescriptionResponse a owl:Class ;
    rdfs:subClassOf ids:ResponseMessage ;
    rdfs:label "Self Description Response"@en ;
    rdfs:comment "Message containing the self-description of an Infrastructure Component."@en.

# Connector-related Messages
# --------------------------

ids:ConnectorAvailableMessage a owl:Class;
    rdfs:subClassOf ids:NotificationMessage ;
    rdfs:label "Connector Available Message"@en ;
    rdfs:comment "Event notifying the recipient(s) about the availability of a new connector. The payload of the message must contain the new connector's self-description."@en.

ids:ConnectorUnavailableMessage a owl:Class;
    rdfs:subClassOf ids:NotificationMessage ;
    rdfs:label "Connector Unavailable Message"@en ;
    rdfs:comment "Event notifying the recipient(s) that a connector will be unavailable and never be available again."@en.

ids:ConnectorTemporarilyUnavailableMessage a owl:Class;
    rdfs:subClassOf ids:NotificationMessage ;
    rdfs:label "Connector Temporarlily Unavailable Message"@en ;
    rdfs:comment "Event notifying the recipient(s) that a connector will be temporarily unavailable and most likely be available again in the future."@en.

ids:ConnectorConfigurationChangeMessage a owl:Class;
    rdfs:subClassOf ids:NotificationMessage ;
    rdfs:label "Connector Configuration Change Message"@en ;
    rdfs:comment "Event notifying the recipient(s) about a connector's configuration change. The payload of the message must contain the updated connector's self-description."@en.

# Participant-related Messages
# ----------------------------

ids:ParticipantCertificateGrantedMessage a owl:Class;
    rdfs:subClassOf ids:NotificationMessage ;
    rdfs:label "Participant Certificate Granted Message"@en ;
    rdfs:comment "Whenever a Participant has been successfully certified by the Certification Body, the Identity Provider can use this message to notify Infrastructure Components."@en.

ids:ParticipantCertificateUnavailableMessage a owl:Class;
    rdfs:subClassOf ids:NotificationMessage ;
    rdfs:label "Participant Certificate Unavailable Message"@en ;
    rdfs:comment "Indicates that a (previously certified) Participant is no more certified. This could happen, for instance, if the Certification Body revokes a granted certificate or if the certificate just expires."@en.

ids:ParticipantCertificateSuspendedMessage a owl:Class;
    rdfs:subClassOf ids:NotificationMessage ;
    rdfs:label "Participant Certificate Suspended Message"@en ;
    rdfs:comment "Event notifying the recipient(s) that a Participant is temporarily no more certified."@en.

ids:ParticipantInformationChangedMessage a owl:Class;
    rdfs:subClassOf ids:NotificationMessage ;
    rdfs:label "Participant Information Changed Message"@en ;
    rdfs:comment "Event notifying the recipient(s) that information describing this Participant has changed. This event is mainly intended for information describing the Participant that is NOT a direct subject of the certification process."@en.

# Broker Messages
# ---------------

ids:BrokerQueryScope a owl:Class;
    rdfs:label "RejectionReason"@en ;
    rdfs:comment "Class of scopes that may limit the space of broker query results."@en.

ids:BrokerQueryMessage a owl:Class;
    rdfs:subClassOf ids:QueryMessage;
    rdfs:label "Broker Query Message"@en ;
    rdfs:comment "Query command intended to be consumed by a Broker."@en.

ids:brokerQueryScope a owl:ObjectProperty;
    rdfs:label "brokerQueryScope"@en;
    rdfs:domain ids:BrokerQueryMessage;
    rdfs:range ids:BrokerQueryScope;
    rdfs:comment "The scope of a query defined in a BrokerQuery message."@en.

ids:QueryLanguage a owl:Class;
    rdfs:label "QueryLanguage"@en ;
    rdfs:comment "Class of query languages in which query strings may be formalized."@en.

ids:queryLanguage a owl:ObjectProperty;
    rdfs:domain ids:BrokerQueryMessage;
    rdfs:range ids:QueryLanguage;
    rdfs:label "queryLanguage"@en;
    rdfs:comment "If queryPayloadType refers to a query string, this property specifies the language of the query."@en.

# Contract Negotiation
# --------------------

ids:ContractRequestMessage a owl:Class ;
    rdfs:subClassOf ids:RequestMessage ;
    rdfs:label "Contract Request Message"@en;
    rdfs:comment "Message containing a suggested content contract (as offered by the data consumer to the data provider) in the associated payload (which is an instance of ContractRequest).";
    idsm:validation [
        idsm:forProperty ids:baseContractOffer;
        idsm:constraint idsm:NotNull;
    ].

ids:baseContractOffer a owl:ObjectProperty;
    rdfs:label "Base Contract Offer"@en ;
    idsm:referenceByUri true;
    rdfs:domain ids:ContractRequestMessage;
    rdfs:range ids:ContractOffer;
    rdfs:comment "The basic offered contract that the contract request message refers to."@en.

ids:ContractOfferMessage a owl:Class ;
    rdfs:subClassOf ids:NotificationMessage ;
    rdfs:label "Contract Offer Message"@en;
    rdfs:comment "Message containing a offered content contract (as offered by the data provider to the data consumer) in the associated payload (which is an instance of ContractOffer).".

ids:ContractAgreementMessage a owl:Class ;
    rdfs:subClassOf ids:ResponseMessage;
    rdfs:label "Contract Agreement Message"@en;
    rdfs:comment "Message containing a contract with resource access modalities on which two parties have agreed."@en.

ids:ContractRejectionMessage a owl:Class ;
    rdfs:subClassOf ids:RejectionMessage;
    rdfs:label "Contract Rejection Message"@en;
    rdfs:comment "Message indicating rejection of a contract."@en.

ids:contractRejectionReason a owl:DatatypeProperty;
    rdfs:label "Contract Rejection Reason"@en ;
    rdfs:domain ids:ContractRejectionMessage;
    rdfs:range rdf:PlainLiteral;
    rdfs:comment "Human-readable text describing the reason for contract rejection."@en.

# Security-related Messages
# -------------------------

ids:AccessTokenRequest a owl:Class ;
    rdfs:subClassOf ids:RequestMessage ;
    rdfs:label "Access Token Request"@en;
    rdfs:comment "Message requesting an access token. This is intended for point-to-point communication with, e.g., Brokers."@en.

ids:AccessTokenResponse a owl:Class ;
    rdfs:subClassOf ids:ResponseMessage ;
    rdfs:label "Access Token Response"@en;
    rdfs:comment "Response to an access token request, intended for point-to-point communication."@en.

# Resource Exchange
# -----------------

ids:ArtifactAvailableMessage a owl:Class ;
    rdfs:subClassOf ids:NotificationMessage ;
    rdfs:label "Artifact Available Message"@en;
    rdfs:comment "Message indicating availability of a specific artifact."@en;
    idsm:validation [
        idsm:forProperty ids:availableArtifact;
        idsm:constraint idsm:NotNull;
    ].

ids:availableArtifact rdf:type owl:DatatypeProperty ;
    idsm:referenceByUri true;
    rdfs:domain ids:ArtifactAvailableMessage;
    rdfs:range ids:Artifact ;
    rdfs:label "Available Artifact"@en ;
    rdfs:comment "References a new artifact from an availability indication."@en.

ids:InvokeOperationMessage a owl:Class ;
    rdfs:subClassOf ids:RequestMessage ;
    rdfs:label "Invoke Operation Message"@en;
    rdfs:comment "Message requesting the recipient to invoke a specific operation."@en;
    idsm:validation [
        idsm:forProperty ids:operationReference;
        idsm:constraint idsm:NotNull;
    ];
    idsm:validation [
        idsm:forProperty ids:operationParameterization;
        idsm:constraint idsm:NotNull;
    ].

ids:operationReference rdf:type owl:DatatypeProperty ;
    idsm:referenceByUri true;
    rdfs:domain ids:InvokeOperationMessage ;
    rdfs:range ids:Operation ;
    rdfs:label "Operation Reference"@en ;
    rdfs:comment "References the operation to be invoked on the recipient's side."@en.

ids:operationParameterization rdf:type owl:DatatypeProperty ;
    rdfs:domain ids:InvokeOperationMessage ;
    rdfs:range ids:ParameterAssignment ;
    rdfs:label "Operation Parameterization"@en ;
    rdfs:comment "Parameter assignment of the invoked operation's input parameters."@en.

ids:RequestInProcessMessage a owl:Class ;
    rdfs:subClassOf ids:NotificationMessage;
    rdfs:label "Request In Process Message"@en;
    rdfs:comment "Notification that a request has been accepted and is being processed."@en;
    idsm:validation [
        idsm:forProperty ids:correlationMessage;
        idsm:constraint idsm:NotNull;
    ].

ids:MessageProcessedNotification a owl:Class ;
    rdfs:subClassOf ids:NotificationMessage;
    rdfs:label "Message Processed"@en;
    rdfs:comment "Notification that a message has been successfully processed (i.e. not ignored or rejected)."@en;
    idsm:validation [
        idsm:forProperty ids:correlationMessage;
        idsm:constraint idsm:NotNull;
    ].

ids:OperationResultMessage  a owl:Class ;
    rdfs:subClassOf ids:MessageProcessedNotification;
    rdfs:label "Operation Result Message"@en;
    rdfs:comment "Message indicating that the result of a former InvokeOperation message is available. May transfer the result data in its associated payload section."@en.

ids:ArtifactRequestMessage a owl:Class ;
    rdfs:subClassOf ids:RequestMessage ;
    rdfs:label "Retrieve Artifact"@en;
    rdfs:comment "Message asking for retrieving the specified Artifact as the payload of an ArtifactResponse message."@en;
    idsm:validation [
        idsm:forProperty ids:requestedArtifact;
        idsm:constraint idsm:NotNull;
    ].

ids:requestedArtifact rdf:type owl:DatatypeProperty ;
    idsm:referenceByUri true;
    rdfs:domain ids:ArtifactRequestMessage;
    rdfs:range ids:Artifact ;
    rdfs:label "Requested Artifact"@en ;
    rdfs:comment "References an artifact in the context of a request."@en.

ids:ArtifactResponseMessage a owl:Class ;
    rdfs:subClassOf ids:ResponseMessage;
    rdfs:label "Artifact Response"@en;
    rdfs:comment "Message that follows up a RetrieveArtifact Message and contains the Artifact's data in the payload section."@en.
