@prefix owl: <http://www.w3.org/2002/07/owl#> .
@prefix rdfs: <http://www.w3.org/2000/01/rdf-schema#> .
@prefix xsd: <http://www.w3.org/2001/XMLSchema#> .
@prefix dct: <http://purl.org/dc/terms/> .
@prefix ids: <https://w3id.org/idsa/core/> .
@prefix idsm: <https://w3id.org/idsa/metamodel/> .

# Classes
# -------

ids:SecurityProfile a owl:Class;
    rdfs:subClassOf ids:CustomSecurityProfile ;
    rdfs:label "SecurityProfile"@en ;
    rdfs:comment "Set of security guarantees claimed by a Connector. Connectors may asses their mutual technical reliability and trustworthiness by evaluating each otherâ€™s security profile."@en .
    # .. specifies several security aspects expressing the minimum requirements a Data Consumer must meet to be granted access to the Data Endpoints exposed by a providing Connector.

ids:CustomSecurityProfile a owl:Class;
    rdfs:label "CustomSecurityProfile"@en;
    rdfs:comment "Specialized security profile that is composed of user-defined security guarantees";
    idsm:validation [
        idsm:forProperty ids:securityGuarantee;
        idsm:relationType idsm:OneToMany;
    ].

ids:SecurityGuarantee
    a owl:Class;
    rdfs:label "Security guarantee"@en ;
    rdfs:comment "Security guarantee claimed by a security profile."@en.

# Properties
# ----------

ids:securityGuarantee
    a owl:ObjectProperty;
    rdfs:domain ids:CustomSecurityProfile;
    rdfs:range ids:SecurityGuarantee;
    rdfs:label "Security guarantee"@en;
    idsm:labelPluralForm "securityGuarantees"@en;
    rdfs:comment "Reference to a security guarantee supported by given profile."@en.